FreydSSA/Terminator/Fun/Subst.lean
@@ -1,7 +1,7 @@
 import FreydSSA.Terminator.Fun.Basic
 import FreydSSA.Term.Fun.Subst
 
--- TODO: SubstCons variants? Friends?
+-- TODO: label-by-label substitution...
 
 variable {φ : Type u₁} {ν : Type u₂} {κ : Type u₃} {α : Type u₄} [Φ : InstSet φ (Ty α)]
   [Φc : CohInstSet φ (Ty α)]
@@ -213,3 +213,214 @@ def UTerminator.FWf'.subst {Γ : FCtx ν (Ty α)} {t : UTerminator φ ν κ}
 def UTerminator.FWf.subst {Γ : FCtx ν (Ty α)} {t : UTerminator φ ν κ}
   (hσ : Γ.Subst σ Δ) (dt : t.FWf Δ L) : (L' : FLCtx κ ν (Ty α)) × (t.rewrite σ).FWfM Γ L' × (L'.Subst σ L)
   := dt.factor.subst hσ
+
+-- TODO: casts to subst, minimization
+
+inductive FLCtx.SubstConsBot
+  : WithBot (FLabel ν (Ty α)) → USubst φ ν →  WithBot (FLabel ν (Ty α)) → Finset ν → Type _
+  | bot (σ Γ N) : SubstConsBot ⊥ σ Γ N
+  | subst {Γ Δ : FLabel ν (Ty α)} (hσ : FCtx.SubstCons Γ.live σ Δ.live N) (hparam : Γ.param = Δ.param) : SubstConsBot (↑Γ) σ (↑Δ) N
+
+-- TODO: composition, other such nonsense
+
+-- Consider: per-κ cons-ness
+def FLCtx.SubstCons (L : FLCtx κ ν (Ty α)) (σ : USubst φ ν) (K : FLCtx κ ν (Ty α)) (N : Finset ν)
+  := ∀x, SubstConsBot (L x) σ (K x) N
+
+-- TODO: composition, other such nonsense
+
+inductive FLCtx.PSubstConsBot
+  : WithBot (FLabel ν (Ty α)) → USubst φ ν →  WithBot (FLabel ν (Ty α)) → Finset ν → Type _
+  | bot (σ N) : PSubstConsBot ⊥ σ ⊥ N
+  | subst {Γ Δ : FLabel ν (Ty α)} (hσ : FCtx.SubstCons Γ.live σ Δ.live N) (hparam : Γ.param = Δ.param) : PSubstConsBot (↑Γ) σ (↑Δ) N
+
+theorem FLCtx.PSubstConsBot.bot_mp {Γ : WithBot (FLabel ν (Ty α))} {σ : USubst φ ν} {Δ : WithBot (FLabel ν (Ty α))}
+  (hσ : PSubstConsBot Γ σ Δ N) : Γ = ⊥ → Δ = ⊥
+  := λh => by cases hσ <;> simp at *
+
+theorem FLCtx.PSubstConsBot.bot_mpr {Γ : WithBot (FLabel ν (Ty α))} {σ : USubst φ ν} {Δ : WithBot (FLabel ν (Ty α))}
+  (hσ : PSubstConsBot Γ σ Δ N) : Δ = ⊥ → Γ = ⊥
+  := λh => by cases hσ <;> simp at *
+
+theorem FLCtx.PSubstConsBot.is_some_mp {Γ : WithBot (FLabel ν (Ty α))} {σ : USubst φ ν} {Δ : WithBot (FLabel ν (Ty α))}
+  (hσ : PSubstConsBot Γ σ Δ N) : Γ.isSome → Δ.isSome
+  := λh => by cases hσ <;> simp [Option.isSome] at *
+
+theorem FLCtx.PSubstConsBot.is_some_mpr {Γ : WithBot (FLabel ν (Ty α))} {σ : USubst φ ν} {Δ : WithBot (FLabel ν (Ty α))}
+  (hσ : PSubstConsBot Γ σ Δ N) : Δ.isSome → Γ.isSome
+  := λh => by cases hσ <;> simp [Option.isSome] at *
+
+theorem FLCtx.PSubstConsBot.param_eq {Γ : FLabel ν (Ty α)} {σ : USubst φ ν} {Δ : FLabel ν (Ty α)}
+  (hσ : @PSubstConsBot _ ν α Φ _ (↑Γ) σ (↑Δ) N) : Γ.param = Δ.param
+  := by cases hσ; assumption
+
+def FLCtx.PSubstConsBot.wkExit {Γ : WithBot (FLabel ν (Ty α))} {σ : USubst φ ν} {Δ Δ' : WithBot (FLabel ν (Ty α))}
+  (hσ : PSubstConsBot Γ σ Δ N) (w : Δ ≤ Δ') : SubstConsBot Γ σ Δ' N
+  := match hσ, Δ' with
+  | bot _ _, _ => SubstConsBot.bot _ _ _
+  | subst hσ hparam, ⊥ => by simp at w
+  | subst hσ hparam, some Δ' =>
+    have w := FLabel.Wk.of_le_coe w;
+    SubstConsBot.subst (hσ.wkExit w.live) (hparam.trans w.param)
+
+def FLCtx.PSubstConsBot.toSubstConsBot
+  {Γ : WithBot (FLabel ν (Ty α))} {σ : USubst φ ν} {Δ : WithBot (FLabel ν (Ty α))}
+  : PSubstConsBot Γ σ Δ N → SubstConsBot Γ σ Δ N
+  | bot _ _ => SubstConsBot.bot _ _ _
+  | subst hσ A => SubstConsBot.subst hσ A
+
+-- Consider: per-κ cons-ness
+def FLCtx.PSubstCons (L : FLCtx κ ν (Ty α)) (σ : USubst φ ν) (K : FLCtx κ ν (Ty α)) (N : Finset ν)
+  := ∀x, PSubstConsBot (L x) σ (K x) N
+
+theorem FLCtx.PSubstCons.bot_mp {L : FLCtx κ ν (Ty α)} {σ : USubst φ ν} {K : FLCtx κ ν (Ty α)}
+  (hσ : L.PSubstCons σ K N) (x : κ) : L x = ⊥ → K x = ⊥
+  := (hσ x).bot_mp
+
+theorem FLCtx.PSubstCons.bot_mpr {L : FLCtx κ ν (Ty α)} {σ : USubst φ ν} {K : FLCtx κ ν (Ty α)}
+  (hσ : L.PSubstCons σ K N) (x : κ) : K x = ⊥ → L x = ⊥
+  := (hσ x).bot_mpr
+
+theorem FLCtx.PSubstCons.is_some_mp {L : FLCtx κ ν (Ty α)} {σ : USubst φ ν} {K : FLCtx κ ν (Ty α)}
+  (hσ : L.PSubstCons σ K N) (x : κ) : (L x).isSome → (K x).isSome
+  := (hσ x).is_some_mp
+
+theorem FLCtx.PSubstCons.is_some_mpr {L : FLCtx κ ν (Ty α)} {σ : USubst φ ν} {K : FLCtx κ ν (Ty α)}
+  (hσ : L.PSubstCons σ K N) (x : κ) : (K x).isSome → (L x).isSome
+  := (hσ x).is_some_mpr
+
+theorem FLCtx.PSubstCons.some_trg {L : FLCtx κ ν (Ty α)} {σ : USubst φ ν} {K : FLCtx κ ν (Ty α)}
+  (hσ : L.PSubstCons σ K N) (x : κ) (Γ : FLabel ν (Ty α)) : L x = some Γ → Σ'Δ, K x = some Δ
+  := λh => ⟨(K x).get (hσ.is_some_mp x (by simp [h])), by simp⟩
+
+def FLCtx.PSubstCons.lsup
+  {L₁ L₂ : FLCtx κ ν (Ty α)} {σ : USubst φ ν} {K₁ K₂ : FLCtx κ ν (Ty α)}
+  (hσ₁ : L₁.PSubstCons σ K₁ N) (hσ₂ : L₂.PSubstCons σ K₂ N) (hL : L₁.Cmp L₂) : (L₁.lsup L₂).PSubstCons σ (K₁.lsup K₂) N
+  := λx => by
+    simp only [lsup_app, lsup_bot]
+    split
+    . rename_i he
+      split
+      . exact hσ₂ x
+      . rename_i c
+        exact (c $ hσ₁.bot_mp _ he).elim
+      . rename_i he' _
+        simp [hσ₁.bot_mp _ he] at he'
+    . rename_i he c
+      split
+      . rename_i he'
+        exact (c $ hσ₁.bot_mpr _ he').elim
+      . exact hσ₁ x
+      . rename_i he'
+        simp [hσ₂.bot_mp _ he] at he'
+    . rename_i Γ₁ Γ₂ hLe₁ hLe₂
+      split
+      . rename_i he
+        simp [hσ₁.bot_mpr _ he] at hLe₁
+      . rename_i he _
+        simp [hσ₂.bot_mpr _ he] at hLe₂
+      . rename_i Δ₁ Δ₂ hKe₁ hKe₂
+        let h₁ := hKe₁ ▸ hLe₁ ▸ hσ₁ x;
+        let h₂ := hKe₂ ▸ hLe₂ ▸ hσ₂ x;
+        have hL := hLe₁ ▸ hLe₂ ▸ hL x
+        cases h₁ with
+        | subst hσ hparam =>
+          cases h₂ with
+          | subst hσ' hparam' =>
+            constructor
+            apply hσ.lsup hσ'
+            cases hL with
+            | both c => exact c.live
+            exact hparam
+
+-- theorem FCtx.Subst.cmp_label {Γ Δ Γ' Δ' : FLabel ν (Ty α)} {σ : USubst φ ν}
+--   (hσ : Γ.live.Subst σ Δ.live) (hσ' : Γ'.live.Subst σ Δ'.live) (hΓ : Γ.Cmp Γ') : Δ.Cmp Δ'
+--   := ⟨sorry, sorry⟩
+
+theorem FLCtx.PSubstConsBot.cmp
+  {Γ Δ Γ' Δ' : WithBot (FLabel ν (Ty α))} {σ : USubst φ ν}
+  (hσ : PSubstConsBot Γ σ Δ N) (hσ' : PSubstConsBot Γ' σ Δ' N') (hΓ : FLCtx.CmpBot Γ Γ') : FLCtx.CmpBot Δ Δ'
+  := by
+    cases hσ with
+    | bot => constructor
+    | subst hΔ hp => cases hσ' with
+      | bot => constructor
+      | subst hΔ' hp' =>
+        cases hΓ with
+        | both hΓ =>
+          constructor
+          constructor
+          exact hΔ.cmp hΔ' hΓ.live
+          rw [<-hp, <-hp', hΓ.param]
+
+theorem FLCtx.PSubstCons.cmp
+  {L₁ L₂ : FLCtx κ ν (Ty α)} {σ : USubst φ ν} {K₁ K₂ : FLCtx κ ν (Ty α)}
+  (hσ₁ : L₁.PSubstCons σ K₁ N) (hσ₂ : L₂.PSubstCons σ K₂ N') (hL : L₁.Cmp L₂) : K₁.Cmp K₂
+  := λx => (hσ₁ x).cmp (hσ₂ x) (hL x)
+
+def FLCtx.PSubstCons.toSubstCons {L : FLCtx κ ν (Ty α)} {σ : USubst φ ν} {K : FLCtx κ ν (Ty α)}
+  (hσ : L.PSubstCons σ K N) : L.SubstCons σ K N
+  := λx => (hσ x).toSubstConsBot
+
+def FCtx.SubstCons.toPSingleton {Γ : FCtx ν (Ty α)} {σ : USubst φ ν} {Δ : FCtx ν (Ty α)}
+  (x : κ) (hσ : Γ.SubstCons σ Δ N) (param : Ty α) : (Γ.toSingleton x param).PSubstCons σ (Δ.toSingleton x param) N
+  := λy => by
+    if h : y = x then
+      simp only [toSingleton, h, FLCtx.singleton_app, ↓reduceIte]
+      constructor
+      assumption
+      rfl
+    else
+      simp only [toSingleton, h, FLCtx.singleton_app, ↓reduceIte]
+      constructor
+
+-- BUG: another spurious unused variable warning. Something something "is water part of the essence of bread" something something
+theorem FCtx.LWkBot.psubstCons_cmp₂ {Γ : FCtx ν (Ty α)} {Δ Ξ M M' : WithBot (FLabel ν (Ty α))} {σ : USubst φ ν}
+  (hΔ : Γ.LWkBot Δ) (hΞ : Γ.LWkBot Ξ) (_hΔ' : FLCtx.PSubstConsBot Δ σ M N) (_hΞ' : FLCtx.PSubstConsBot Ξ σ M' N')
+  (hM : FLCtx.CmpBot M M')
+  : FLCtx.CmpBot Δ Ξ
+  := match hΔ, hΞ with
+  | bot, _ => by constructor
+  | _, bot => by constructor
+  | wk A w, wk A' w' => by
+    constructor
+    cases M with
+    | none => cases _hΔ'
+    | some M =>
+      cases _hΔ'
+      cases _hΞ'
+      constructor
+      exact w.cmp₂ w'
+      cases hM
+      rename_i h
+      cases h
+      aesop
+
+theorem FCtx.LWk.psubstCons_cmp₂ {L K M M' : FLCtx κ ν (Ty α)} {Γ : FCtx ν (Ty α)} {σ : USubst φ ν}
+  (hL : Γ.LWk L) (hK : Γ.LWk K) (hLM : L.PSubstCons σ M N) (hKM : K.PSubstCons σ M' N') (hM : M.Cmp M')
+  : L.Cmp K
+  := λx => (hL x).psubstCons_cmp₂ (hK x) (hLM x) (hKM x) (hM x)
+
+def UTerminator.FWfM.substCons {Γ : FCtx ν (Ty α)} {t : UTerminator φ ν κ}
+  (hσ : Γ.SubstCons σ Δ N)
+  : t.FWfM Δ L → (L' : FLCtx κ ν (Ty α)) × (t.rewrite σ).FWfM Γ L' × (L'.PSubstCons σ L N)
+  | br _ de rfl => ⟨_, br _ (de.subst hσ.toSubst) rfl, hσ.toPSingleton _ _⟩
+  | ite de ds dt h rfl =>
+    let ⟨_, ds', σs'⟩ := ds.substCons hσ;
+    let ⟨_, dt', σt'⟩ := dt.substCons hσ;
+    let ls' := ds'.trgLEq.toLWk;
+    let lt' := dt'.trgLEq.toLWk;
+    let hc := ls'.psubstCons_cmp₂ lt' σs' σt' h;
+    ⟨_, ite (de.subst hσ.toSubst) ds' dt' hc rfl, σs'.lsup σt' hc⟩
+
+def FLCtx.PSubstCons.wkExit {L : FLCtx κ ν (Ty α)} {σ : USubst φ ν} {K : FLCtx κ ν (Ty α)}
+  {K' : FLCtx κ ν (Ty α)} (hσ : L.PSubstCons σ K N) (w : K.Wk K') : L.SubstCons σ K' N
+  := λx => (hσ x).wkExit (w x)
+
+def UTerminator.FWf'.substCons {Γ : FCtx ν (Ty α)} {t : UTerminator φ ν κ}
+  (hσ : Γ.SubstCons σ Δ N) (dt : t.FWf' Δ L) : (L' : FLCtx κ ν (Ty α)) × (t.rewrite σ).FWfM Γ L' × (L'.SubstCons σ L N)
+  := let dt' := dt.FWfM.substCons hσ; ⟨dt'.1, dt'.2.1, dt'.2.2.wkExit dt.wk⟩
+
+def UTerminator.FWf.substCons {Γ : FCtx ν (Ty α)} {t : UTerminator φ ν κ}
+  (hσ : Γ.SubstCons σ Δ N) (dt : t.FWf Δ L) : (L' : FLCtx κ ν (Ty α)) × (t.rewrite σ).FWfM Γ L' × (L'.SubstCons σ L N)
+  := dt.factor.substCons hσ
